more changes

Pipeline/Impl.v
@@ -1,10 +1,10 @@
 Require Import Kami.AllNotations.
 
-Require Import ProcKami.FU.
+Require Import StdLibKami.Fifo.Ifc.
 
+Require Import ProcKami.Pipeline.Mem.Ifc.
 Require Import ProcKami.Pipeline.Mem.Impl.
 
-Require Import ProcKami.Pipeline.Ifc.
 Require Import ProcKami.Pipeline.Decoder.
 Require Import ProcKami.Pipeline.RegReader.
 Require Import ProcKami.Pipeline.InputXform.
@@ -12,13 +12,19 @@ Require Import ProcKami.Pipeline.Executer.
 Require Import ProcKami.Pipeline.Commit.
 Require Import ProcKami.Pipeline.ConfigReader.
 
-Require Import StdLibKami.Fifo.Ifc.
-Require Import StdLibKami.Fetcher.Ifc.
+Require Import ProcKami.Pipeline.Ifc.
 
-(* TODO create the instance *)
-Section Pipeline.
+Require Import ProcKami.MemOps.
+Require Import ProcKami.MemOpsFuncs.
+
+Require Import ProcKami.FU.
+Require Import ProcKami.Device.
+
+Section Impl.
   Context {procParams: ProcParams}.
-  Context {func_units : list FUEntry}.
+  Context (func_units : list FUEntry).
+  Context (deviceTree: @DeviceTree procParams).
+  Context (memIfcParams: @Mem.Ifc.Params).
 
   Definition CommitPkt := (STRUCT_TYPE {
                          "completePc" :: Maybe FU.VAddr ;
@@ -27,51 +33,66 @@ Section Pipeline.
                          "exception"  :: Maybe Exception })%kami_expr.
 
   Local Instance tokenFifoParams
-    :  FifoParams
-    := {|
-         StdLibKami.Fifo.Ifc.name := @^"tokenFifo";
-         StdLibKami.Fifo.Ifc.k := Void;
+    :  Fifo.Ifc.Params
+    := {| Fifo.Ifc.name := @^"tokenFifo";
+          Fifo.Ifc.k := Void;
+          Fifo.Ifc.size := 1;
        |}.
 
-  Local Instance fetchAddrExFifoParams
-    :  FifoParams
-    := {|
-         StdLibKami.Fifo.Ifc.name := @^"fetchAddrExFifo";
-         StdLibKami.Fifo.Ifc.k := Maybe Exception;
+  Local Instance fetchAddrExceptionFifoParams
+    :  Fifo.Ifc.Params
+    := {| Fifo.Ifc.name := @^"fetchAddrExceptionFifo";
+          Fifo.Ifc.k := Maybe Exception;
+          Fifo.Ifc.size := 1;
        |}.
 
-  Local Instance fetchInstExFifoParams
-    :  FifoParams
-    := {|
-         StdLibKami.Fifo.Ifc.name := @^"fetchInstExFifo";
-         StdLibKami.Fifo.Ifc.k := Maybe Exception;
+  Local Instance fetchInstExceptionFifoParams
+    :  Fifo.Ifc.Params
+    := {| Fifo.Ifc.name := @^"fetchInstExceptionFifo";
+          Fifo.Ifc.k := Maybe Exception;
+          Fifo.Ifc.size := 2 ^ fetcherLgSize;
        |}.
 
   Local Instance decExecFifoParams
-    :  FifoParams
-    := {|
-         StdLibKami.Fifo.Ifc.name := @^"decExecFifo";
-         StdLibKami.Fifo.Ifc.k := CommitPkt;
+    :  Fifo.Ifc.Params
+    := {| Fifo.Ifc.name := @^"decExecFifo";
+          Fifo.Ifc.k := CommitPkt;
+          Fifo.Ifc.size := 1;
        |}.
 
-  Context (tokenFifo: Fifo tokenFifoParams).
-  Context (fetchAddrExFifo: Fifo fetchAddrExFifoParams).
-  Context (fetchInstExFifo: Fifo fetchInstExFifoParams).
-  Context (decExecFifo: Fifo decExecFifoParams).
+  Local Definition tokenFifo: @Fifo.Ifc.Ifc tokenFifoParams.
+    refine (@Fifo.Impl.impl _ {| Fifo.Impl.sizePow2 := _ ;
+                                 Fifo.Impl.regArray := @RegArray.RegList.impl _ |}).
+    abstract auto.
+  Defined.
+
+  Local Definition fetchAddrExceptionFifo: @Fifo.Ifc.Ifc fetchAddrExceptionFifoParams.
+    refine (@Fifo.Impl.impl _ {| Fifo.Impl.sizePow2 := _ ;
+                                 Fifo.Impl.regArray := @RegArray.RegList.impl _ |}).
+    abstract auto.
+  Defined.
+
+  Local Definition decExecFifo: @Fifo.Ifc.Ifc decExecFifoParams.
+    refine (@Fifo.Impl.impl _ {| Fifo.Impl.sizePow2 := _ ;
+                                 Fifo.Impl.regArray := @RegArray.RegList.impl _ |}).
+    abstract auto.
+  Defined.
+
+  Local Definition fetchInstExceptionFifo: @Fifo.Ifc.Ifc fetchInstExceptionFifoParams.
+    refine (@Fifo.Impl.impl _ {| Fifo.Impl.sizePow2 := _ ;
+                                 Fifo.Impl.regArray := @RegArray.RegList.impl _ |}).
+    abstract (simpl; rewrite Natlog2_up_pow2; auto).
+  Defined.
 
   Section memInterfaceSizeParams.
-    Context (memInterfaceSizeParams : MemInterfaceSizeParams).
-    Variable ty: Kind -> Type.
-
     Local Open Scope kami_action.
     Local Open Scope kami_expr.
 
-    (* TODO: LLEE: modify to respond differently based on the response tag. *)
-    Definition handleMemRes ty
-      (res : ty (@ArbiterMemUnitRes procParams memInterfaceSizeParams))
+    Definition memCallback ty
+               (res: ty (@MemResp _ memIfcParams))
       :  ActionT ty Void
       := System [
-           DispString _ "[Mem.handleMemRes] res: ";
+           DispString _ "[memCallback] res: ";
            DispHex #res;
            DispString _ "\n"
          ];
@@ -80,11 +101,11 @@ Section Pipeline.
                                  "tag" ::= (IF #oldOptCommit @% "data" @% "execCxt" @% "memHints" @% "data" @% "isFrd"
                                              then $FloatRegTag
                                              else $IntRegTag);
-                                 "data"  ::= #res @% "resp" @% "data"
+                                 "data"  ::= #res @% "res" @% "data"
                                };
          LET newUpdatePkt
            :  ExecUpdPkt
-           <- IF #res @% "resp" @% "valid"
+           <- IF #res @% "res" @% "valid"
                 then #oldOptCommit @% "data" @% "execUpd" @%["val1" <- Valid #wb]
                 else #oldOptCommit @% "data" @% "execUpd";
          LET commitPkt
@@ -92,7 +113,7 @@ Section Pipeline.
            <- #oldOptCommit @% "data" @%["execUpd" <- #newUpdatePkt];
          LETA cxtCfg: ContextCfgPkt <- readConfig _;
          System [
-           DispString _ "[Mem.handleMemRes] commit pkt: ";
+           DispString _ "[memCallback] commit pkt: ";
            DispHex #commitPkt;
            DispString _ "\n"
          ];
@@ -105,9 +126,8 @@ Section Pipeline.
     Local Close Scope kami_expr.
     Local Close Scope kami_action.
   End memInterfaceSizeParams.
-
-  Context {memInterfaceParams: @MemInterfaceParams procParams}.
-  Context {memInterface: @MemInterface procParams memInterfaceParams}.
+  
+  Definition mem := @Mem.Impl.impl  _ deviceTree _ memCallback.
 
   Section ty.
     Variable ty: Kind -> Type.
@@ -128,7 +148,6 @@ Section Pipeline.
         Retv );
       Retv.
 
-    (* Stage 1 *)
     Local Definition sendPcRule: ActionT ty Void :=
       LETA cxtCfg: ContextCfgPkt <- readConfig _;
       LETA isEmpty <- @Fifo.Ifc.isEmpty _ tokenFifo _;
@@ -138,269 +157,177 @@ Section Pipeline.
         System [
           DispString _ "[sendPcRule]\n"
         ];
-        LET prefetchVAddr
-          :  FU.VAddr
-          <- Fetcher.Ifc.toFullVAddr (@Fetcher.Ifc.toShortVAddr fetcherParams ty #pc);
-        System [
-          DispString _ "[sendPcRule] prefetch vaddr: ";
-          DispHex #prefetchVAddr;
-          DispString _ "\n"
-        ];
-        LETA optPAddrEx
-          :  Maybe (PktWithException PAddr)
-          <- @memTranslate _ _ memInterface _ #cxtCfg $VmAccessInst #prefetchVAddr;
-        If #optPAddrEx @% "valid"
+        LETA optPAddrDevOffsetException
+          :  Maybe (PktWithException (@PAddrDevOffset _ deviceTree))
+          <- @memTranslate _ _ _ mem _ #cxtCfg $VmAccessInst (getMemOpCode memOps _ Lw) #pc;
+        If #optPAddrDevOffsetException @% "valid"
         then (
-          LET val : Maybe Exception <- (#optPAddrEx @% "data" @% "snd");
-          LETA _ <- @Fifo.Ifc.enq _ fetchAddrExFifo _ val;
-          If !(#optPAddrEx @% "data" @% "snd" @% "valid")
-          then
-            LET req 
-              <- STRUCT { 
-                   "mode"  ::= #cxtCfg @% "mode";
-                   "paddr" ::= Valid (#optPAddrEx @% "data" @% "fst");
-                   "vaddr" ::= #prefetchVAddr
-                 };
-            LETA res : Bool <- @MemInterface.Ifc.doPrefetch _ _ memInterface _ req;
-            If #res
-              then
-                LETA _ <- @Fifo.Ifc.deq _ tokenFifo _;
-                Retv;
-            Retv
-          else
+          LET val : Maybe Exception <- (#optPAddrDevOffsetException @% "data" @% "snd");
+          LETA _ <- @Fifo.Ifc.enq _ fetchAddrExceptionFifo _ val;
+          LET inReq : PAddrDevOffsetVAddr deviceTree <- STRUCT { "memReq" ::= #optPAddrDevOffsetException @% "data" @% "fst" ;
+                                                                 "vaddr" ::= #pc } ;
+          LET req <- STRUCT { "inReq" ::= #inReq ;
+                              "sendReq?" ::= !(#optPAddrDevOffsetException @% "data" @% "snd" @% "valid") };
+          LETA accepted : Bool <- @Mem.Ifc.fetcherSendAddr _ _ _ mem ty req;
+          If #accepted
+          then (
             LETA _ <- @Fifo.Ifc.deq _ tokenFifo _;
-            Retv
-          as _;
-          Retv);
+            Retv );
+          Retv );
         Retv);
       Retv.
 
-    (* Stage 2 *)
-    Local Definition transferTlbFetchExceptionRule: ActionT ty Void :=
-      LETA optPAddrEx <- @Fifo.Ifc.first _ fetchAddrExFifo _;
-      LETA is_full <- @Fifo.Ifc.isFull _ fetchInstExFifo _;
-      If (!#is_full && #optPAddrEx @% "valid")
+    Local Definition transferMmuFetchExceptionRule: ActionT ty Void :=
+      LETA optPAddrException <- @Fifo.Ifc.first _ fetchAddrExceptionFifo _;
+      LETA isFull <- @Fifo.Ifc.isFull _ fetchInstExceptionFifo _;
+      If (!#isFull && #optPAddrException @% "valid")
       then (
         System [
-          DispString _ "[transferTlbFetchExceptionRule]\n"
+          DispString _ "[transferMmuFetchExceptionRule]\n"
         ];
-        LETA _ <- @Fifo.Ifc.deq _ fetchAddrExFifo _;
-        LET pAddrEx <- #optPAddrEx @% "data";    
-        @Fifo.Ifc.enq _ fetchInstExFifo _ pAddrEx
+        LETA _ <- @Fifo.Ifc.deq _ fetchAddrExceptionFifo _;
+        LET pAddrException <- #optPAddrException @% "data";    
+        @Fifo.Ifc.enq _ fetchInstExceptionFifo _ pAddrException
       );
       Retv.
 
-    (* Stage 3 *)
     Local Definition decodeExecRule: ActionT ty Void :=
-      LETA optPAddrEx : Maybe (Maybe Exception) <- @Fifo.Ifc.first _ fetchInstExFifo _;
+      LETA optInstException : Maybe (Maybe Exception) <- @Fifo.Ifc.first _ fetchInstExceptionFifo _;
       LETA isFull <- @Fifo.Ifc.isFull _ decExecFifo _;
-      LETA cxtCfg: ContextCfgPkt <- readConfig _;
-      LETA fetchInst: Maybe Ifc.Fetcher.Ifc.OutRes <- MemInterface.Ifc.firstFetchInstruction memInterface _;
-      LET compPc: Maybe FU.VAddr <- STRUCT { "valid" ::= #fetchInst @% "data" @% "notComplete" ;
-                                          "data"  ::= #fetchInst @% "data" @% "vaddr"};
-      If #compPc @% "valid" && !#isFull
-      then
-        (* I.A. fetch incomplete. we need to fetch again. *)
-        System [
-          DispString _ "[decodeExecRule] pc: ";
-          DispHex #compPc;
-          DispString _ "\n"
+      LETA fetchInst: Maybe FetchOutput <- @Mem.Ifc.fetcherFirst _ _ _ mem _;
+      System [
+        DispString _ "[decodeExecRule] FetchInst: \n";
+        DispHex #fetchInst;
+        DispString _ "[decodeExecRule] Exception: ";
+        DispHex #optInstException;
+        DispString _ "[decodeExecRule] isFull: ";
+        DispHex #isFull;
+        DispString _ "\n"
         ];
-        LET def
-          :  CommitPkt
-          <- STRUCT {
-               "completePc" ::= #compPc ;
-               "execCxt"    ::= $$(getDefaultConst ExecContextPkt) ;
-               "execUpd"    ::= $$(getDefaultConst ExecUpdPkt);
-               "exception"  ::= (Invalid: Maybe Exception @# ty)
-             };
-        LETA _ <- @Fifo.Ifc.enq _ decExecFifo _ def;
-        LETA _ <- @Fifo.Ifc.deq _ fetchInstExFifo _;
-        Retv
-      else
-        (* I.B. fetch complete. *)
-        If #optPAddrEx @% "valid"
-        then
-          LETA _ <- MemInterface.Ifc.deqFetchInstruction memInterface _;
-          If #optPAddrEx @% "data" @% "valid" && !#isFull
-          then
-            (* II.A. Exception occured during fetch. *)
-            LET def
-              :  CommitPkt
-              <- STRUCT {
-                   "completePc" ::= #compPc ;
-                   "execCxt"    ::= $$(getDefaultConst ExecContextPkt) ;
-                   "execUpd"    ::= $$(getDefaultConst ExecUpdPkt);
-                   "exception"  ::= #optPAddrEx @% "data"
-                 };
-            LETA _ <- @Fifo.Ifc.enq _ decExecFifo _ def;
-            LETA _ <- @Fifo.Ifc.deq _ fetchInstExFifo _;
-            Retv
-          else
-            (* II.B. Fetched instruction *)
-            If #fetchInst @% "valid" && !#isFull
-            then
-              System [
-                DispString _ "[decodeExecRule] optPAddrEx: ";
-                DispHex #optPAddrEx;
-                DispString _ "\n";
-                DispString _ "[decodeExecRule] fetchInst: ";
-                DispHex #fetchInst;
-                DispString _ "\n"
-              ];
-              LET isImmErr : Bool <- mem_error (#fetchInst @% "data" @% "info");
-              LET startingException
-                :  Maybe Exception
-                <- STRUCT {
-                     "valid"
-                       ::= (#optPAddrEx @% "data" @% "valid" ||
-                            #isImmErr ||
-                            !(#fetchInst @% "data" @% "noErr"));
-                     "data"
-                       ::= IF #optPAddrEx @% "data" @% "valid"
-                             then #optPAddrEx @% "data" @% "data"
-                             else
-                               IF #isImmErr
-                                 then
-                                   getMemErrorException
-                                     ($VmAccessInst)
-                                     (#fetchInst @% "data" @% "info")
-                                 else $InstAccessFault
-                   };
-              System [
-                DispString _ "[decodeExecRule] starting exception: ";
-                DispHex #startingException;
-                DispString _ "\n"
-              ];
-              LET fetchPkt
-                :  FetchPkt
-                <- STRUCT {
-                     "pc"             ::= #fetchInst @% "data" @% "vaddr" ;
-                     "inst"           ::= #fetchInst @% "data" @% "inst" ;
-                     "compressed?"    ::= #fetchInst @% "data" @% "compressed?" ;
-                     "exceptionUpper" ::= #fetchInst @% "data" @% "errUpper?"
-                   };
-              System [
-                DispString _ "[decodeExecRule] fetch pkt: ";
-                DispHex #fetchPkt;
-                DispString _ "\n"
-              ];
-              LETA decoderPkt
-                <- decoderWithException #cxtCfg
-                     (STRUCT {
-                        "fst" ::= #fetchPkt;
-                        "snd" ::= #startingException});
-              System [
-                DispString _ "[decodeExecRule] decoder pkt: ";
-                DispHex #decoderPkt;
-                DispString _ "\n"
-              ];
-              LETA execContextPkt
-                <- readerWithException (func_units := func_units)
-                     (#fetchInst @% "data" @% "vaddr")
-                     #cxtCfg #decoderPkt (#fetchPkt @% "compressed?")
-                     (#fetchPkt @% "exceptionUpper");
-              System [
-                DispString _ "[decodeExecRule] execute context pkt: ";
-                DispHex #execContextPkt;
-                DispString _ "\n"
-              ];
-              LETA inputPkt <- inputXformWithException #cxtCfg (#decoderPkt @% "fst") #execContextPkt;
-              System [
-                DispString _ "[decodeExecRule] input pkt: ";
-                DispHex #inputPkt;
-                DispString _ "\n"
-              ];
-              LETA execUpdPkt <- execWithException #inputPkt;
-              System [
-                DispString _ "[decodeExecRule] execute update pkt: ";
-                DispHex #execUpdPkt;
-                DispString _ "\n"
-              ];
-              LET initDef
-                :  CommitPkt
-                <- STRUCT {
-                     "completePc" ::= #compPc ;
-                     "execCxt"    ::= #execContextPkt @% "fst" ;
-                     "execUpd"    ::= #execUpdPkt @% "fst";
-                     "exception"  ::= #execUpdPkt @% "snd"
-                   };
-              If #execContextPkt @% "fst" @% "memHints" @% "valid" &&
-                 #execUpdPkt @% "fst" @% "val2" @% "valid" &&
-                 !(#execUpdPkt @% "snd" @% "valid")
-              then
+      If (!#isFull && #optInstException @% "valid" && #fetchInst @% "valid")
+      then (
+        LETA context: ContextCfgPkt <- readConfig _;
+        LET compPc: Maybe FU.VAddr <- STRUCT { "valid" ::= #fetchInst @% "data" @% "notComplete?" ;
+                                               "data"  ::= #fetchInst @% "data" @% "vaddr"};
+        If (#compPc @% "valid" || #optInstException @% "data" @% "valid") (* I.A. fetch incomplete or exception. we need to fetch again. *)
+        then (
+          LET enqVal : CommitPkt <- STRUCT { "completePc" ::= #compPc ;
+                                             "execCxt"    ::= $$(getDefaultConst ExecContextPkt) ;
+                                             "execUpd"    ::= $$(getDefaultConst ExecUpdPkt);
+                                             "exception"  ::= (#optInstException @% "data": Maybe Exception @# ty) };
+          System [
+            DispString _ "[decodeExecRule] Incomplete\n"
+            ];
+          LETA _ <- @Fifo.Ifc.enq _ decExecFifo _ enqVal;
+          LETA _ <- @Fifo.Ifc.deq _ fetchInstExceptionFifo _;
+          LETA _ <- @Mem.Ifc.fetcherDeq _ _ _ mem _;
+          Retv )
+        else ( (* I.B. fetch complete and no exception. *)
+          LET fetchPkt: FetchPkt <- STRUCT {
+                                        "pc"             ::= #fetchInst @% "data" @% "vaddr" ;
+                                        "inst"           ::= #fetchInst @% "data" @% "inst" ;
+                                        "compressed?"    ::= #fetchInst @% "data" @% "compressed?" ;
+                                        "exceptionUpper" ::= #fetchInst @% "data" @% "errUpper?" };
+          System [
+            DispString _ "[decodeExecRule] fetch pkt: ";
+            DispHex #fetchPkt;
+            DispString _ "\n"
+          ];
+          LETA decoderPkt <- decoderWithException #context (STRUCT { "fst" ::= #fetchPkt;
+                                                                     "snd" ::= #optInstException @% "data"});
+          System [
+            DispString _ "[decodeExecRule] decoder pkt: ";
+            DispHex #decoderPkt;
+            DispString _ "\n"
+          ];
+          LETA execContextPkt <-
+            readerWithException
+              (func_units := func_units) (#fetchInst @% "data" @% "vaddr") #context #decoderPkt (#fetchPkt @% "compressed?") (#fetchPkt @% "exceptionUpper");
+          System [
+            DispString _ "[decodeExecRule] execute context pkt: ";
+            DispHex #execContextPkt;
+            DispString _ "\n"
+          ];
+          LETA inputPkt <- inputXformWithException #context (#decoderPkt @% "fst") #execContextPkt;
+          System [
+            DispString _ "[decodeExecRule] input pkt: ";
+            DispHex #inputPkt;
+            DispString _ "\n"
+          ];
+          LETA execUpdPkt <- execWithException #inputPkt;
+          System [
+            DispString _ "[decodeExecRule] execute update pkt: ";
+            DispHex #execUpdPkt;
+            DispString _ "\n"
+          ];
+          LET enqVal: CommitPkt <- STRUCT { "completePc" ::= #compPc ;
+                                            "execCxt"    ::= #execContextPkt @% "fst" ;
+                                            "execUpd"    ::= #execUpdPkt @% "fst";
+                                            "exception"  ::= #execUpdPkt @% "snd" };
+          If (#execContextPkt @% "fst" @% "memHints" @% "valid" (* Memory *)
+              && #execUpdPkt @% "fst" @% "val2" @% "valid" (* Not failed Store Conditional - could be other reasons *)
+              && !(#execUpdPkt @% "snd" @% "valid")) (* No Exception *)
+          then (
+            System [
+              DispString _ "[decodeExecRule] sending request to translate memory request addr.\n"
+            ];
+            LET vaddr: FU.VAddr <- xlen_sign_extend Xlen (#context @% "xlen") (#execUpdPkt @% "fst" @% "val2" @% "data" @% "data" : Bit Rlen @# ty);
+            LETA mmuResp: Maybe (PktWithException (PAddrDevOffset deviceTree)) <- @memTranslate _ _ _ mem _  #context
+                                                                                                (IF #execContextPkt @% "fst" @% "memHints" @% "data" @% "isSAmo"
+                                                                                                 then $VmAccessSAmo
+                                                                                                 else $VmAccessLoad)
+                                                                                                (#execContextPkt @% "fst" @% "memHints" @% "data" @% "memOp")
+                                                                                                #vaddr;
+            System [
+              DispString _ "[decodeExecRule] memory request MMU res: ";
+              DispHex #mmuResp;
+              DispString _ "\n"
+            ];
+            If #mmuResp @% "valid" (* TLB Hit *)
+            then (
+              If #mmuResp @% "data" @% "snd" @% "valid" (* TLB exception *)
+              then (
+                LET newEnqVal <- #enqVal @%[ "exception" <- #mmuResp @% "data" @% "snd"];
+                LETA _ <- @Fifo.Ifc.enq _ decExecFifo _ newEnqVal;
+                LETA _ <- @Fifo.Ifc.deq _ fetchInstExceptionFifo _;
+                LETA _ <- @Mem.Ifc.fetcherDeq _ _ _ mem _;
+                Retv )
+              else ( (* TLB no exception *)
+                LET memReq: MemReq deviceTree <- STRUCT { "dtag" ::= #mmuResp @% "data" @% "fst" @% "dtag" ;
+                                                          "offset" ::= #mmuResp @% "data" @% "fst" @% "offset" ;
+                                                          "paddr" ::= #mmuResp @% "data" @% "fst" @% "paddr" ;
+                                                          "memOp" ::= #execContextPkt @% "fst" @% "memHints" @% "data" @% "memOp" ;
+                                                          "data" ::= #execUpdPkt @% "fst" @% "val1" @% "data" @% "data"};
+                LET memUnitMemReq: MemUnitMemReq deviceTree <- STRUCT { "tag" ::= $0;
+                                                                        "req" ::= #memReq };
+                LETA accepted: Bool <- @sendMemUnitMemReq _ _ _ mem _ memUnitMemReq;
                 System [
-                  DispString _ "[decodeExecRule] sending tlb request to translate memory request addr.\n"
-                ];
-                LET vaddr: FU.VAddr
-                 <- xlen_sign_extend Xlen
-                      (#cxtCfg @% "xlen")
-                      (#execUpdPkt @% "fst" @% "val2" @% "data" @% "data" : Bit Rlen @# ty);
-                LETA tlbResp
-                  :  Maybe (PktWithException PAddr)
-                  <- @memTranslate _ _ memInterface _  #cxtCfg
-                       (IF #execContextPkt @% "fst" @% "memHints" @% "data" @% "isSAmo"
-                         then $VmAccessSAmo else $VmAccessLoad)
-                       #vaddr;
-                System [
-                  DispString _ "[decodeExecRule] memory request tlb res: ";
-                  DispHex #tlbResp;
+                  DispString _ "[decodeExecRule] memory unit req accepted: ";
+                  DispHex #accepted;
                   DispString _ "\n"
                 ];
-                If #tlbResp @% "valid"
-                then
-                  If #tlbResp @% "data" @% "snd" @% "valid"
-                  then
-                    LET newEnq <- #initDef @%[ "exception" <- #tlbResp @% "data" @% "snd"];
-                    LETA _ <- @Fifo.Ifc.enq _ decExecFifo _ newEnq;
-                    LETA _ <- @Fifo.Ifc.deq _ fetchInstExFifo _;
-                    Retv
-                  else
-                    LETA memReqRet
-                      :  Maybe (Maybe Exception)
-                      <- @sendMemReq _ _ memInterface _
-                           $0
-                           #cxtCfg
-                           (#execContextPkt @% "fst")
-                           (#tlbResp @% "data" @% "fst");
-                    System [
-                      DispString _ "[decodeExecRule] memory imm res: ";
-                      DispHex #memReqRet;
-                      DispString _ "\n"
-                    ];
-                    If #memReqRet @% "valid"
-                    then
-                      If #memReqRet @% "data" @% "valid"
-                      then
-                        LET newEnq <- #initDef @%[ "exception" <- #memReqRet @% "data"];
-                        LETA _ <- @Fifo.Ifc.enq _ decExecFifo _ newEnq;
-                        @Fifo.Ifc.deq _ fetchInstExFifo _
-                      else
-                        LETA _ <- @Fifo.Ifc.enq _ decExecFifo _ initDef;
-                        @Fifo.Ifc.deq _ fetchInstExFifo _
-                      as _;
-                      Retv;
-                    Retv
-                  as _;
-                  Retv;
-                Retv
-              else
-                LETA _ <- @Fifo.Ifc.enq _ decExecFifo _ initDef;
-                LETA _ <- @Fifo.Ifc.deq _ fetchInstExFifo _;
-                Retv
-              as _;
-              Retv;
-            Retv
-            as _;
-          Retv;
-        Retv;
+                If #accepted (* Requrest accepted *)
+                then (
+                  LETA _ <- @Fifo.Ifc.enq _ decExecFifo _ enqVal;
+                  LETA _ <- @Fifo.Ifc.deq _ fetchInstExceptionFifo _ ;
+                  LETA _ <- @Mem.Ifc.fetcherDeq _ _ _ mem _;
+                  Retv ) ;
+                Retv );
+              Retv );
+            Retv )
+          else ( (* Not memory *)
+            LETA _ <- @Fifo.Ifc.enq _ decExecFifo _ enqVal;
+            LETA _ <- @Fifo.Ifc.deq _ fetchInstExceptionFifo _;
+            LETA _ <- @Mem.Ifc.fetcherDeq _ _ _ mem _;
+            Retv );
+          Retv );
+        Retv );
       Retv.
 
-    (* Stage 4 *)
     Local Definition commitRule: ActionT ty Void :=
       Read isWfi : Bool <- @^"isWfi";
       LETA optCommit <- @Fifo.Ifc.first _ decExecFifo _;
-      LETA cxtCfg: ContextCfgPkt <- readConfig _;
+      LETA context: ContextCfgPkt <- readConfig _;
       If #optCommit @% "valid" && !#isWfi 
       then (
         System [
@@ -419,7 +346,7 @@ Section Pipeline.
           If !(#optCommit @% "data" @% "execCxt" @% "memHints" @% "valid") ||
              (#optCommit @% "data" @% "exception" @% "valid")
           then (
-            LETA _ <- commit #cxtCfg (#optCommit @% "data" @% "execCxt") (#optCommit @% "data" @% "execUpd")
+            LETA _ <- commit #context (#optCommit @% "data" @% "execCxt") (#optCommit @% "data" @% "execUpd")
                  (#optCommit @% "data" @% "exception");
             LETA _ <- @Fifo.Ifc.deq _ decExecFifo _;
             LET  tokenFifoVal : Void <- $$(getDefaultConst Void);
@@ -435,33 +362,33 @@ Section Pipeline.
     Local Close Scope kami_action.
   End ty.
 
-  Definition procPipeline
-    :  Pipeline
+  Definition impl
+    :  Ifc
     := {|
-         ProcKami.Pipeline.Ifc.regs
+         Pipeline.Ifc.regs
            := [
-                (@^"initReg",
-                 existT RegInitValT (SyntaxKind Bool)
-                   (Some (SyntaxConst (ConstBool false))))
+                (@^"initReg", existT RegInitValT (SyntaxKind Bool) (Some (SyntaxConst (ConstBool false))))
               ] ++
               @Fifo.Ifc.regs _ tokenFifo ++
-              @Fifo.Ifc.regs _ fetchAddrExFifo ++
-              @Fifo.Ifc.regs _ fetchInstExFifo ;
-         ProcKami.Pipeline.Ifc.regFiles
+              @Fifo.Ifc.regs _ fetchAddrExceptionFifo ++
+              @Fifo.Ifc.regs _ fetchInstExceptionFifo ++
+              @Mem.Ifc.regs _ _ _ mem;
+         Pipeline.Ifc.regFiles
            := @Fifo.Ifc.regFiles _ tokenFifo ++
-              @Fifo.Ifc.regFiles _ fetchAddrExFifo ++
-              @Fifo.Ifc.regFiles _ fetchInstExFifo ;
-         ProcKami.Pipeline.Ifc.tokenStartRule               := tokenStartRule;
-         ProcKami.Pipeline.Ifc.sendPcRule                   := sendPcRule;
-         ProcKami.Pipeline.Ifc.tlbSendMemReqRule            := MemInterface.Ifc.tlbSendMemReqRule memInterface;
-         ProcKami.Pipeline.Ifc.devRouterPollRules           := MemInterface.Ifc.devRouterPollRules memInterface;
-         ProcKami.Pipeline.Ifc.responseToPrefetcherRule     := MemInterface.Ifc.responseToPrefetcherRule memInterface;
-         ProcKami.Pipeline.Ifc.prefetcherTransferRule       := MemInterface.Ifc.prefetcherTransferRule memInterface;
-         ProcKami.Pipeline.Ifc.prefetcherNotCompleteDeqRule := MemInterface.Ifc.prefetcherNotCompleteDeqRule memInterface;
-         ProcKami.Pipeline.Ifc.fetchInstRule                := transferTlbFetchExceptionRule;
-         ProcKami.Pipeline.Ifc.decodeExecRule               := decodeExecRule;
-         ProcKami.Pipeline.Ifc.commitRule                   := commitRule;
-         ProcKami.Pipeline.Ifc.arbiterRule                  := MemInterface.Ifc.arbiterRule memInterface;
+              @Fifo.Ifc.regFiles _ fetchAddrExceptionFifo ++
+              @Fifo.Ifc.regFiles _ fetchInstExceptionFifo ++
+              @Mem.Ifc.regFiles _ _ _ mem;
+         Pipeline.Ifc.tokenStartRule                := tokenStartRule;
+         Pipeline.Ifc.mmuSendReqRule                := Mem.Ifc.mmuSendReqRule mem;
+         Pipeline.Ifc.sendPcRule                    := sendPcRule;
+         Pipeline.Ifc.transferMmuFetchExceptionRule := transferMmuFetchExceptionRule;
+         Pipeline.Ifc.routerPollRules               := Mem.Ifc.routerPollRules mem;
+         Pipeline.Ifc.responseToFetcherRule         := Mem.Ifc.responseToFetcherRule mem;
+         Pipeline.Ifc.fetcherTransferRule           := Mem.Ifc.fetcherTransferRule mem;
+         Pipeline.Ifc.fetcherNotCompleteDeqRule     := Mem.Ifc.fetcherNotCompleteDeqRule mem;
+         Pipeline.Ifc.decodeExecRule                := decodeExecRule;
+         Pipeline.Ifc.commitRule                    := commitRule;
+         Pipeline.Ifc.arbiterResetRule              := Mem.Ifc.arbiterResetRule mem;
        |}.
 
-End Pipeline.
+End Impl.
